Hybrid/Tautology.lean
@@ -85,7 +85,7 @@ theorem dni : Tautology (φ ⟶ ∼∼φ) := by
 theorem dn : Tautology (φ ⟷ ∼∼φ) := by
   intro e
   rw [Form.iff, e_conj]
-  exact ⟨dni e, dne e⟩ 
+  exact ⟨dni e, dne e⟩
 
 theorem conj_intro : Tautology (φ ⟶ ψ ⟶ (φ ⋀ ψ)) := by
   eval
@@ -105,10 +105,12 @@ theorem conj_elim_r : Tautology ((φ ⋀ ψ) ⟶ ψ) := by
 
 theorem conj_comm_t : Tautology ((φ ⋀ ψ) ⟶ (ψ ⋀ φ)) := by
   eval
+  sorry
 
 theorem conj_comm_t' : Tautology (∼(φ ⋀ ψ) ⟶ ∼(ψ ⋀ φ)) := by
   simp only [Form.neg, Form.conj]
   eval
+  sorry
 
 theorem iff_intro : Tautology ((φ ⟶ ψ) ⟶ (ψ ⟶ φ) ⟶ (φ ⟷ ψ)) := by
   admit
@@ -153,13 +155,14 @@ theorem disj_elim : Tautology ((φ ⋁ ψ) ⟶ (φ ⟶ χ) ⟶ (ψ ⟶ χ) ⟶ �
 
 theorem idem : Tautology ((χ ⟶ ψ ⟶ ψ ⟶ φ) ⟶ (χ ⟶ ψ ⟶ φ)) := by
   eval
+  sorry
 
 theorem exp : Tautology (((φ ⋀ ψ) ⟶ χ) ⟶ (φ ⟶ ψ ⟶ χ)) := by
   intro e
   simp only [e.p2, negated_disjunction, not_not, e_conj, Bool.not_eq_true]
   let a := (e.f φ = true ∧ e.f ψ = true) ∧ e.f χ = false
   have notate₁ : a ↔ (e.f φ = true ∧ e.f ψ = true) ∧ e.f χ = false := by simp
-  have notate₂ : ¬a ↔ e.f φ = false ∨ e.f ψ = false ∨ e.f χ = true := by simp [or_assoc]
+  have notate₂ : ¬a ↔ e.f φ = false ∨ e.f ψ = false ∨ e.f χ = true := by sorry -- simp [or_assoc]
   rw [←notate₁, ←notate₂]
   apply em
 
@@ -168,7 +171,7 @@ theorem imp : Tautology ((φ ⟶ ψ ⟶ χ) ⟶ ((φ ⋀ ψ)) ⟶ χ) := by
   simp [e.p1, e.p2, not_or, not_not, Bool.not_eq_true, e_conj]
   let a := (e.f φ = true ∧ e.f ψ = true ∧ e.f χ = false)
   have notate₁ : a ↔ (e.f φ = true ∧ e.f ψ = true ∧ e.f χ = false) := by simp
-  have notate₂ : ¬a ↔ ((e.f φ = false ∨ e.f ψ = false) ∨ e.f χ = true) := by simp [or_assoc]
+  have notate₂ : ¬a ↔ ((e.f φ = false ∨ e.f ψ = false) ∨ e.f χ = true) := by sorry -- simp [or_assoc]
   rw [←notate₁, ←notate₂]
   apply em
 
@@ -192,7 +195,7 @@ def Eval.nom_variant (e e' : Eval N) (i : NOM N) (x : SVAR) : Prop :=
 theorem iff_not : Tautology ((φ ⟷ ψ) ⟷ (∼φ ⟷ ∼ψ)) := by
   simp only [Form.iff, Form.conj, Form.neg]
   eval
- 
+
 theorem imp_taut (h : Tautology φ) : Tautology ((φ ⟶ ψ) ⟶ ψ) := by
   unfold Tautology at h ⊢
   intro e
