lakefile.lean
@@ -5,12 +5,10 @@ package hybrid {
   -- add package configuration options here
 }
 
+@[default_target]
 lean_lib Hybrid {
   -- add library configuration options here
 }
 
-@[default_target]
-lean_lib hybrid
-
 require mathlib from git
-  "https://github.com/leanprover-community/mathlib4.git"
+  "https://github.com/leanprover-community/mathlib4.git"@"v4.13.0"
